src/Parsers/BooleanRecognizer.v
@@ -24,8 +24,7 @@ Section recursive_descent_parser.
       : bool
         := match it with
              | Terminal ch => str ~= [ ch ]
-             | NonTerminal nt => ((is_valid_nonterminal initial_nonterminals_data nt)
-                                   && str_matches_nonterminal nt)%bool
+             | NonTerminal nt => str_matches_nonterminal nt
            end.
 
       Section production.
@@ -76,9 +75,7 @@ Section recursive_descent_parser.
                           (pf : len <= len0),
                      String.string -> bool).
 
-        (** To parse as a given list of [production]s, we must parse
-            as one of the [production]s; we only need to look at the
-            ones labeled by the selection function. *)
+        (** To parse as a given list of [production]s, we must parse as one of the [production]s. *)
         Definition parse_productions'
                    (str : String)
                    (len : nat)
@@ -87,11 +84,10 @@ Section recursive_descent_parser.
         : bool
           := fold_right orb
                         false
-                        (map (option_rect (fun _ => bool) (fun x => x) false)
-                             (map (option_map (parse_production' parse_nonterminal str pf))
-                                  (map (nth_error prods)
-                                       (select_production_rules prods str)))).
+                        (map (parse_production' parse_nonterminal str pf)
+                             prods).
       End productions.
+
 
       Section nonterminals.
         Section step.
@@ -112,36 +108,35 @@ Section recursive_descent_parser.
           : bool.
           Proof.
             refine
-              ((is_valid_nonterminal initial_nonterminals_data nt)
-                 && (parse_productions'
-                       (sumbool_rect
-                          (fun b => forall (str' : String) (len' : nat), len' <= (if b then len else len0) -> String.string -> bool)
-                          (fun _ => (** [str] got smaller, so we reset the valid nonterminals list *)
-                             @parse_nonterminal
-                               (len, nonterminals_length initial_nonterminals_data)
-                               (or_introl _)
-                               initial_nonterminals_data)
-                          (fun _ => (** [str] didn't get smaller, so we cache the fact that we've hit this nonterminal already *)
-                             sumbool_rect
-                               (fun _ => forall (str' : String) (len' : nat), len' <= len0 -> String.string -> bool)
-                               (fun is_valid => (** It was valid, so we can remove it *)
-                                  @parse_nonterminal
-                                    (len0, pred valid_len)
-                                    (or_intror (conj eq_refl _))
-                                    (remove_nonterminal valid nt))
+              (parse_productions'
+                 (sumbool_rect
+                    (fun b => forall (str' : String) (len' : nat), len' <= (if b then len else len0) -> String.string -> bool)
+                    (fun _ => (** [str] got smaller, so we reset the valid nonterminals list *)
+                       @parse_nonterminal
+                         (len, nonterminals_length initial_nonterminals_data)
+                         (or_introl _)
+                         initial_nonterminals_data)
+                    (fun _ => (** [str] didn't get smaller, so we cache the fact that we've hit this nonterminal already *)
+                       sumbool_rect
+                         (fun _ => forall (str' : String) (len' : nat), len' <= len0 -> String.string -> bool)
+                         (fun is_valid => (** It was valid, so we can remove it *)
+                            @parse_nonterminal
+                              (len0, pred valid_len)
+                              (or_intror (conj eq_refl _))
+                              (remove_nonterminal valid nt))
 
-                               (fun _ _ _ _ _ => (** oops, we already saw this nonterminal in the past.  ABORT! *)
-                                  false)
-                               (Sumbool.sumbool_of_bool (negb (EqNat.beq_nat valid_len 0) && is_valid_nonterminal valid nt)))
-                          (lt_dec len len0))
-                       str
-                       (len := len)
-                       (sumbool_rect
-                          (fun b => len <= (if b then len else len0))
-                          (fun _ => le_n _)
-                          (fun _ => _)
-                          (lt_dec len len0))
-                       (Lookup G nt)))%bool;
+                         (fun _ _ _ _ _ => (** oops, we already saw this nonterminal in the past.  ABORT! *)
+                            false)
+                         (Sumbool.sumbool_of_bool (negb (EqNat.beq_nat valid_len 0) && is_valid_nonterminal valid nt)))
+                    (lt_dec len len0))
+                 str
+                 (len := len)
+                 (sumbool_rect
+                    (fun b => len <= (if b then len else len0))
+                    (fun _ => le_n _)
+                    (fun _ => _)
+                    (lt_dec len len0))
+                 (Lookup G nt));
             first [ assumption
                   | simpl;
                     generalize (proj1 (proj1 (Bool.andb_true_iff _ _) is_valid));
