src/Parsers/BooleanRecognizerOptimized.v
@@ -12,7 +12,6 @@ Require Import Fiat.Common.Match.
 Require Import Fiat.Common.List.ListFacts.
 Require Import Fiat.Common.Equality.
 Require Export Fiat.Common.SetoidInstances.
-Require Import Fiat.Common.OptionFacts.
 
 Set Implicit Arguments.
 Local Open Scope string_like_scope.
@@ -39,7 +38,6 @@ Proof.
   f_equal.
   unfold parse_item'.
   destruct a; trivial.
-  rewrite H; reflexivity.
 Qed.
 
 Local Ltac simpl_setoid_rewrite lem :=
@@ -53,18 +51,15 @@ Section recursive_descent_parser.
           {ls : list (String.string * productions Char)}.
   Context {data : @boolean_parser_dataT Char _}.
 
-  Class str_carrier_data (constT varT : Type)
+  Class str_carrier (constT varT : Type)
     := { to_string : constT * varT -> String;
-         of_string_const : String -> constT;
-         of_string_var : String -> varT }.
-  Class str_carrier_ok (constT varT : Type) {SD : str_carrier_data constT varT}
-    := { to_of : forall x, to_string (of_string_const x, of_string_var x) = x;
-         of_const_to : forall x, of_string_const (to_string x) = fst x;
-         of_var_to : forall x, of_string_var (to_string x) = snd x;
-         drop_const : forall x n, of_string_const (drop n x) = of_string_const x;
-         take_const : forall x n, of_string_const (take n x) = of_string_const x }.
+         of_string : String -> constT * varT;
+         to_of : forall x, to_string (of_string x) = x;
+         of_to : forall x, of_string (to_string x) = x;
+         drop_const : forall x n, fst (of_string (drop n x)) = fst (of_string x);
+         take_const : forall x n, fst (of_string (take n x)) = fst (of_string x)}.
 
-  (*Definition str_carrier' (constT varT : Type)
+  Definition str_carrier' (constT varT : Type)
     := { to_string : constT * varT -> StringLike.String
        & { of_string : StringLike.String -> constT * varT
          | (forall x, to_string (of_string x) = x)
@@ -78,46 +73,11 @@ Section recursive_descent_parser.
     refine {| to_string := projT1 strC;
               of_string := proj1_sig (projT2 strC) |};
     apply (proj2_sig (projT2 strC)).
-  Defined.*)
+  Defined.
 
-  Context constT varT {strC : str_carrier_data constT varT} {strCH : str_carrier_ok}.
+  Context constT varT {strC : str_carrier constT varT}.
 
   Local Notation G := (list_to_grammar (nil::nil) ls) (only parsing).
-
-  Local Ltac do_proper_solve_with tac
-    := repeat match goal with
-                | [ |- ?x = ?x ] => reflexivity
-                | [ |- ?x = ?y ] => is_evar x; is_var y; reflexivity
-                | [ |- ?x = false ] => is_evar x; reflexivity
-                | [ |- ?x = true ] => is_evar x; reflexivity
-                | [ |- pointwise_relation _ _ _ _ ] => intro
-                | _ => solve [ tac ]
-                | [ |- _ = fold_left _ _ _ ]
-                  => apply fold_left_f_eq_mor_Proper
-                | [ |- _ = fold_right _ _ _ ]
-                  => apply fold_right_f_eq_mor_Proper
-                | [ |- _ = map _ _ ]
-                  => apply map_Proper_eq; [ intro | ]
-                | [ |- _ = option_rect ?P _ _ _ ]
-                  => apply option_rect_Proper
-                | [ |- _ = option_map _ _ ]
-                  => apply option_map_Proper; [ intro | ]
-                | [ |- _ = nth_error _ _ ]
-                  => apply f_equal2
-                | [ |- _ = select_production_rules _ _ ]
-                  => apply f_equal2
-                | [ |- orb _ _ = orb _ _ ]
-                  => apply f_equal2
-                | [ |- andb _ _ = andb _ _ ]
-                  => apply f_equal2
-                | [ |- ?f ?x ?y = bool_rect (fun _ => ?P) ?a ?b ?c ]
-                  => is_evar f;
-                    refine (_ : bool_rect (fun _ => P) (_ x y) (_ x y) (_ x y) = bool_rect (fun _ => P) a b c); cbv beta;
-                    apply f_equal3
-                | [ |- ?f ?x = ?f' ?x ] => is_evar f; is_var f'; is_var x; reflexivity
-                | [ |- ?f ?x ?y = ?f' ?x ?y ] => is_evar f; is_var f'; is_var x; is_var y; reflexivity
-                | [ |- ?f ?x ?y = orb ?x ?y ] => is_evar f; is_var x; is_var y; reflexivity
-              end.
 
   Definition parse_nonterminal_opt'
              (str : String)
@@ -167,79 +127,25 @@ Section recursive_descent_parser.
                          | _ => reflexivity
                          | [ |- appcontext[match ?e with left _ => _ | right _ => _ end] ]
                            => destruct e
-                         | [ |- ?e = andb (is_valid_nonterminal _ _) _ ]
-                           => subst e;
-                             apply f_equal;
-                             match goal with
-                               | [ |- ?e' = _ ]
-                                 => set (e := e')
-                             end
                        end;
-                rewrite !map_map;
-                do_proper_solve_with idtac;
-                rewrite (parse_production'_respectful H');
+                setoid_rewrite (parse_production'_respectful H');
                 reflexivity ] ];
       [
-      | let e2 := fresh in
-        evar (e2 : bool);
-        refine (eq_trans _ (_ : andb _ e2 = _));
-          [
-          | apply f_equal;
-            repeat match goal with
-                     | _ => rewrite !map_map
-                     | _ => setoid_rewrite option_rect_option_map
-                     | _ => setoid_rewrite (fun ls => eq_sym (@fold_symmetric _ orb Bool.orb_assoc Bool.orb_comm false ls))
-                     | _ => progress cbv beta
-                     | [ |- appcontext[?f (fold_right (fun x acc => bool_rect (fun _ => _) _ acc _) _ ?ls)] ]
-                       => let h := head f in
-                          not constr_eq h (@eq);
-                            rewrite (fun init => @f_fold_right_bool_rect _ _ _ (fun k => f k) init ls)
-                     | [ |- appcontext[?f _ (fold_right (fun x acc => bool_rect (fun _ => _) _ acc _) _ ?ls)] ]
-                       => let h := head f in
-                          not constr_eq h (@eq);
-                            rewrite (fun extra_arg init => @f_fold_right_bool_rect _ _ _ (fun k => f extra_arg k) init ls)
-                     | [ |- appcontext[fold_right (fun str_t else_case => bool_rect (fun _ => ?A -> ?B) (@?a str_t) else_case (@?b str_t))] ]
-                       => setoid_rewrite (@fold_right_fun_bool_rect _ _ _ a b)
-                     | [ |- appcontext[?f (fold_right (fun x acc => bool_rect (fun _ => _) _ acc _) _ ?ls)] ]
-                       => let h := head f in
-                          not constr_eq h (@eq);
-                            simpl_setoid_rewrite (fun init => @f_fold_right_bool_rect _ _ _ (fun k => f k) init ls)
-                     | [ |- appcontext[?f _ (fold_right (fun x acc => bool_rect (fun _ => _) _ acc _) _ ?ls)] ]
-                       => let h := head f in
-                          not constr_eq h (@eq);
-                            simpl_setoid_rewrite (fun extra_arg init => @f_fold_right_bool_rect _ _ _ (fun k => f extra_arg k) init ls)
-                     | [ |- appcontext G[fold_right (fun str_t else_case s => bool_rect (fun _ => ?T) (@?a str_t) (else_case s) (@?b str_t s))] ]
-                       => etransitivity;
-                         [
-                         | solve [
-                               do_proper_solve_with
-                                 ltac:(symmetry;
-                                       match goal with
-                                         | [ |- fold_right (fun str_t else_case s => bool_rect (fun _ => ?T') (@?a' str_t) (else_case s) (@?b' str_t s)) _ _ _ = _ ]
-                                           => exact (@fold_right_fun
-                                                       _ _ _
-                                                       (fun str_t else_cases s => bool_rect (fun _ => T') (a' str_t) else_cases (b' str_t s))
-                                                       _ _ _)
-                                       end)
-                         ] ]
-                     | [ |- appcontext[fold_right (fun str_t else_case => bool_rect (fun _ => ?A -> ?B) (@?a str_t) else_case (@?b str_t))] ]
-                       => etransitivity;
-                         [
-                         | solve [
-                               do_proper_solve_with
-                                 ltac:(symmetry;
-                                       lazymatch goal with
-                                       | [ |- fold_right (fun str_t else_case => bool_rect (fun _ => ?A -> ?B) (@?a str_t) else_case (@?b str_t)) _ _ _ = _ ]
-                                         => exact (@fold_right_fun_bool_rect _ _ _ a b _ _ _)
-                                       | [ |- appcontext[fold_right (fun str_t else_case => bool_rect (fun _ => ?A -> ?B) (@?a str_t) else_case (@?b str_t))] ]
-                                         => fail 1
-                                       | _ => reflexivity
-                                       end) ] ]
-                   end;
-            subst e2; reflexivity ];
-          subst e2;
-          try subst pp; simpl;
-          subst e'; instantiate; reflexivity ];
+      | repeat match goal with
+                 | _ => progress simpl
+                 | _ => setoid_rewrite (fun ls => eq_sym (@fold_symmetric _ orb Bool.orb_assoc Bool.orb_comm false ls))
+                 | _ => setoid_rewrite Bool.orb_false_r
+                 | [ |- appcontext[fold_right (fun str_t else_case s => bool_rect (fun _ => ?T) (@?a str_t) (else_case s) (@?b str_t s))] ]
+                   => simpl_setoid_rewrite (@fold_right_fun _ _ _ (fun str_t else_cases s => bool_rect (fun _ => T) (a str_t) else_cases (b str_t s)))
+                 | [ |- appcontext[?f (fold_right (fun x acc => bool_rect (fun _ => _) _ acc _) _ ?ls) ?x] ]
+                   => simpl_setoid_rewrite (fun init => @f_fold_right_bool_rect _ _ _ (fun k => f k x) init ls)
+                 | [ |- appcontext[?f (fold_right (fun x acc => bool_rect (fun _ => _) _ acc _) _ ?ls)] ]
+                   => simpl_setoid_rewrite (fun init => @f_fold_right_bool_rect _ _ _ f init ls)
+                 | [ |- appcontext[?f _ (fold_right (fun x acc => bool_rect (fun _ => _) _ acc _) _ ?ls)] ]
+                   => simpl_setoid_rewrite (fun extra_arg init => @f_fold_right_bool_rect _ _ _ (fun k => f extra_arg k) init ls)
+               end;
+        try subst pp; simpl;
+        subst e'; instantiate; reflexivity ];
       cbv beta iota zeta delta [bool_rect sumbool_rect];
       simpl;
       subst e; instantiate.
@@ -249,7 +155,7 @@ Section recursive_descent_parser.
   Lemma take_drop_helper n ms x
   : take n (fold_right drop (to_string x) ms)
     = to_string (fst x,
-                 of_string_var (take n (fold_right drop (to_string x) ms))).
+                 snd (of_string (take n (fold_right drop (to_string x) ms)))).
   Proof.
     rewrite <- (rev_involutive ms).
     rewrite fold_left_rev_right.
@@ -263,12 +169,12 @@ Section recursive_descent_parser.
       end.
       apply f_equal.
       apply injective_projections.
-      { rewrite take_const, !of_const_to; reflexivity. }
-      { rewrite !of_var_to; simpl; reflexivity. } }
-    { pose proof (IHms n (let x' := (drop a (to_string (x, y))) in (of_string_const x', of_string_var x'))) as IHms'.
+      { rewrite take_const, !of_to; reflexivity. }
+      { rewrite !of_to; simpl; reflexivity. } }
+    { pose proof (IHms n (of_string (drop a (to_string (x, y))))) as IHms'.
       rewrite to_of in IHms'.
-      rewrite IHms'; clear IHms'; simpl.
-      rewrite drop_const, !of_var_to, !of_const_to; simpl.
+      rewrite IHms'; clear IHms'.
+      rewrite drop_const, !of_to; simpl.
       reflexivity. }
   Qed.
 
@@ -292,40 +198,40 @@ Section recursive_descent_parser.
                          (z : String)
                      => @?f a' x y z)
                     ?v1 ?v2 ?str ?v4 ?v5 ?v6 ]
-        => idtac;
-          let f' := constr:(fun const_str
+        => let f' := constr:(fun const_str
                                  (a' : T0)
                                  (x : forall a'' : T0, R a'' a' -> T1 -> varT -> T2' a'')
                                  (y : T1)
                                  (z : varT)
                              => f a' (fun a'' rwf t1 str'
-                                      => x a'' rwf t1 (of_string_var str'))
+                                      => x a'' rwf t1 (snd (of_string str')))
                                   y (to_string (const_str, z))) in
-          let vstr' := constr:(of_string_var str) in
-          let f'h := fresh "f0" in
-          let fh := fresh "f1" in
-          set (f'h := f');
-            set (fh := f);
-            let GT := constr:(Fix
-                                wf
-                                (fun (a : T0) => T1 -> varT -> T2)
-                                (f'h (of_string_const str))
-                                v1 v2 vstr' v4 v5 v6
-                              = Fix
-                                  wf
-                                  (fun (a : T0) => T1 -> String -> T2)
-                                  fh
-                                  v1 v2 str v4 v5 v6) in
-            refine (_ : GT); change GT;
-            let H := fresh in
-            assert (H : forall a b vstr' d e f0,
-                          Fix wf (fun (a : T0) => T1 -> varT -> T2) (f'h (of_string_const str)) a b vstr' d e f0
-                          = Fix wf (fun (a : T0) => T1 -> String -> T2) fh a b (to_string (of_string_const str, vstr')) d e f0);
-              [ let a := fresh in intro a; induction (wf a) as [?? IH]
-              | specialize (fun a b => H a b (of_string_var str));
-                rewrite to_of in H;
-                rewrite <- H;
-                reflexivity ]
+           let vstr' := constr:(snd (of_string str)) in
+           let f'h := fresh "f0" in
+           let fh := fresh "f1" in
+           set (f'h := f');
+             set (fh := f);
+             let GT := constr:(Fix
+                                 wf
+                                 (fun (a : T0) => T1 -> varT -> T2)
+                                 (f'h (fst (of_string str)))
+                                 v1 v2 vstr' v4 v5 v6
+                               = Fix
+                                   wf
+                                   (fun (a : T0) => T1 -> String -> T2)
+                                   fh
+                                   v1 v2 str v4 v5 v6) in
+             refine (_ : GT); change GT;
+             let H := fresh in
+             assert (H : forall a b vstr' d e f0,
+                           Fix wf (fun (a : T0) => T1 -> varT -> T2) (f'h (fst (of_string str))) a b vstr' d e f0
+                           = Fix wf (fun (a : T0) => T1 -> String -> T2) fh a b (to_string (fst (of_string str), vstr')) d e f0);
+               [ let a := fresh in intro a; induction (wf a) as [?? IH]
+               | specialize (fun a b => H a b (snd (of_string str)));
+                 rewrite <- surjective_pairing in H;
+                 rewrite to_of in H;
+                 rewrite <- H;
+                 reflexivity ]
     end.
     intros.
     rewrite !Fix5_eq;
@@ -336,15 +242,14 @@ Section recursive_descent_parser.
                | _ => progress intros
                | [ |- ?x = ?x ] => reflexivity
                | [ |- fold_right _ _ _ = fold_right _ _ _ ]
-                 => apply fold_right_f_eq_mor_Proper; [ intros ?? | | ]
+                 => apply fold_right_f_eq_mor; [ intros ?? | | ]
                | [ |- (match ?x with _ => _ end) = (match ?x with _ => _ end) ]
                  => destruct x eqn:?
                | [ |- (match ?x with _ => _ end) _ _ _ _ = (match ?x with _ => _ end) _ _ _ _ ]
                  => destruct x eqn:?
-               | [ H : of_string_const _ = ?x |- context[?x] ] => rewrite <- H
+               | [ H : fst (of_string _) = ?x |- context[?x] ] => rewrite <- H
                | [ |- fold_left _ _ _ = fold_left _ _ _ ]
                  => rewrite <- !fold_left_rev_right
-               | _ => progress do_proper_solve_with idtac
                | [ |- rev _ = rev _ ]
                  => apply f_equal
                | [ |- map _ ?ls = map _ ?ls ]
@@ -353,15 +258,13 @@ Section recursive_descent_parser.
                  => apply f_equal2
                | [ |- context[(fst ?x, snd ?x)] ]
                  => rewrite <- surjective_pairing
-               | [ |- context[to_string (of_string_const _, of_string_var _)] ]
+               | [ |- context[to_string (of_string _)] ]
                  => rewrite to_of
-               | [ |- context[of_string_const (to_string _)] ]
-                 => rewrite of_const_to
-               | [ |- context[of_string_var (to_string _)] ]
-                 => rewrite of_var_to
+               | [ |- context[of_string (to_string _)] ]
+                 => rewrite of_to
                | [ H : context[(fst ?x, snd ?x)] |- _ ]
                  => rewrite <- surjective_pairing in H
-               | [ H : context[to_string (of_string_const _, of_string_var _)] |- _ ]
+               | [ H : context[to_string (of_string _)] |- _ ]
                  => rewrite to_of in H
                | [ |- parse_production' _ _ _ _ = parse_production' _ _ _ _ ]
                  => apply parse_production_drop_ext with (ms := nil); intros
@@ -400,7 +303,7 @@ End recursive_descent_parser.
     judgmentally [const_data * variable_data], and [take] and [drop]
     judgmentally preserve the constant data. *)
 
-(*Ltac solve_default_str_carrier :=
+Ltac solve_default_str_carrier :=
   match goal with |- str_carrier _ _ => idtac end;
   eapply str_carrier_default; hnf; simpl;
   match goal with |- { to_string : _ * _ -> string * _ & _ } => idtac end;
@@ -411,4 +314,3 @@ End recursive_descent_parser.
     solve [ repeat split ].
 
 Hint Extern 1 (str_carrier _ _) => solve_default_str_carrier : typeclass_instances.
-*)
