src/Parsers/ParserImplementation.v
@@ -2,14 +2,13 @@
 Require Export Fiat.Parsers.ParserInterface.
 Require Import Fiat.Parsers.ContextFreeGrammar.
 Require Import Fiat.Parsers.ContextFreeGrammarProperties.
+Require Import Fiat.Parsers.BooleanRecognizer Fiat.Parsers.BooleanRecognizerCorrect.
 Require Import Fiat.Parsers.Splitters.RDPList.
 Require Import Fiat.Parsers.BaseTypes Fiat.Parsers.CorrectnessBaseTypes.
 Require Import Fiat.Parsers.StringLike.Core.
 Require Import Fiat.Parsers.MinimalParseOfParse.
-Require Import Fiat.Parsers.BooleanRecognizer Fiat.Parsers.BooleanRecognizerCorrect.
 Require Import Fiat.Common.
 Require Import Fiat.Common.Equality.
-Require Import Fiat.Common.List.ListFacts.
 
 Set Implicit Arguments.
 
@@ -22,139 +21,98 @@ Section implementation.
   Local Instance parser_data : @boolean_parser_dataT Char _ :=
     { predata := rdp_list_predata (G := G);
       split_string_for_production it its str
-      := splits_for splitter str it its;
-      select_production_rules prods str
-      := rules_for splitter str prods }.
+      := splits_for splitter str it its }.
 
   Local Instance parser_completeness_data : @boolean_parser_completeness_dataT' Char _ G parser_data
-    := { split_string_for_production_complete len0 valid str pf nt Hvalid := _;
-         select_production_rules_complete len0 valid str pf nt Hvalid := _ }.
+    := { split_string_for_production_complete str0 valid str pf nt Hvalid := _ }.
   Proof.
-    { unfold is_valid_nonterminal in Hvalid; simpl in Hvalid.
-      unfold rdp_list_is_valid_nonterminal in Hvalid; simpl in Hvalid.
-      hnf in Hvalid.
-      apply Equality.list_in_bl in Hvalid; [ | apply @Equality.string_bl ].
-      generalize (fun it its n pf pit pits prefix H' pitH pitsH => @splits_for_complete Char G splitter str it its n pf (ex_intro _ nt (ex_intro _ prefix (conj Hvalid H'))) pit pits pitH pitsH).
-      clear Hvalid.
-      induction (G nt) as [ | x xs IHxs ].
-      { intros; constructor. }
-      { intro H'.
-        Opaque split_string_for_production.
+    unfold is_valid_nonterminal in Hvalid; simpl in Hvalid.
+    unfold rdp_list_is_valid_nonterminal in Hvalid; simpl in Hvalid.
+    hnf in Hvalid.
+    apply Equality.list_in_bl in Hvalid; [ | apply @Equality.string_bl ].
+    generalize (fun it its n pf pit pits prefix H' pitH pitsH => @splits_for_complete Char G splitter str it its n pf (ex_intro _ nt (ex_intro _ prefix (conj Hvalid H'))) pit pits pitH pitsH).
+    clear Hvalid.
+    induction (G nt) as [ | x xs IHxs ].
+    { intros; constructor. }
+    { intro H'.
+      Opaque split_string_for_production.
+      simpl.
+      Transparent split_string_for_production.
+      split;
+        [ clear IHxs
+        | apply IHxs;
+          intros; eapply H'; try eassumption; [ right; eassumption ] ].
+      specialize (fun prefix it its H n pf pit pits pitH pitsH => H' it its n pf pit pits prefix (or_introl H) pitH pitsH).
+      clear -H'.
+      induction x as [ | it its IHx ].
+      { simpl; constructor. }
+      { Opaque split_string_for_production.
         simpl.
         Transparent split_string_for_production.
         split;
-          [ clear IHxs
-          | apply IHxs;
-            intros; eapply H'; try eassumption; [ right; eassumption ] ].
-        specialize (fun prefix it its H n pf pit pits pitH pitsH => H' it its n pf pit pits prefix (or_introl H) pitH pitsH).
-        clear -H'.
-        induction x as [ | it its IHx ].
-        { simpl; constructor. }
-        { Opaque split_string_for_production.
-          simpl.
-          Transparent split_string_for_production.
-          split;
-            [ clear IHx
-            | apply IHx;
-              intros; subst; eapply (H' (_::_)); try eassumption; reflexivity ].
-          specialize (H' nil it its eq_refl).
-          hnf.
-          intros [ n [ pit pits ] ]; simpl in * |- .
-          destruct (Compare_dec.le_ge_dec n (length str)).
-          { exists n; repeat split; eauto.
-            specialize (fun pf =>
-                          H' _ pf
-                             (projT1 (parse_of_item__of__minimal_parse_of_item pit))
-                             (projT1 (parse_of_production__of__minimal_parse_of_production pits))).
-            apply H'; eauto.
-            { erewrite <- parse_of_item_respectful_refl.
-              eapply expand_forall_parse_of_item;
-                [ ..
-                | rewrite parse_of_item_respectful_refl;
-                  exact (projT2 (parse_of_item__of__minimal_parse_of_item pit)) ];
-                try reflexivity; simpl.
-              simpl; intros ????? H0.
-              unfold rdp_list_is_valid_nonterminal in *.
-              apply list_in_bl in H0; [ | apply @string_bl ]; assumption. }
-            { erewrite <- parse_of_production_respectful_refl.
-              eapply expand_forall_parse_of_production;
-                [ ..
-                | rewrite parse_of_production_respectful_refl;
-                  exact (projT2 (parse_of_production__of__minimal_parse_of_production pits)) ];
-                try reflexivity; simpl.
-              simpl; intros ????? H0.
-              unfold rdp_list_is_valid_nonterminal in *.
-              apply list_in_bl in H0; [ | apply @string_bl ]; assumption. } }
-          { exists (length str).
-            specialize (H' (length str) (reflexivity _)).
-            pose proof (fun H => expand_minimal_parse_of_item (str' := take (length str) str) (or_introl (reflexivity _)) (reflexivity _) (or_introl (reflexivity _)) H pit) as pit'; clear pit.
-            pose proof (fun H => expand_minimal_parse_of_production (str' := drop (length str) str) (or_introl (reflexivity _)) (reflexivity _) (or_introl (reflexivity _)) H pits) as pits'; clear pits.
-            refine ((fun ret => let pit'' := pit' (fst (snd ret)) in
-                                let pits'' := pits' (snd (snd ret)) in
-                                ((H' (projT1 (fst (fst ret) pit'')) (projT1 (snd (fst ret) pits'')) (projT2 (fst (fst ret) pit'')) (projT2 (snd (fst ret) pits'')), pit''), pits'')) _); repeat split.
-            { intro p.
-              exists (projT1 (@parse_of_item__of__minimal_parse_of_item Char splitter G _ _ _ _ _ p)).
-              erewrite <- parse_of_item_respectful_refl.
-              eapply expand_forall_parse_of_item;
-                [ ..
-                | rewrite parse_of_item_respectful_refl;
-                  exact (projT2 (parse_of_item__of__minimal_parse_of_item p)) ];
-                try reflexivity; simpl.
-              simpl; intros ????? H0.
-              unfold rdp_list_is_valid_nonterminal in *.
-              apply list_in_bl in H0; [ | apply @string_bl ]; assumption. }
-            { intro p.
-              exists (projT1 (@parse_of_production__of__minimal_parse_of_production Char splitter G _ _ _ _ _ p)).
-              erewrite <- parse_of_production_respectful_refl.
-              eapply expand_forall_parse_of_production;
-                [ ..
-                | rewrite parse_of_production_respectful_refl;
-                  exact (projT2 (parse_of_production__of__minimal_parse_of_production p)) ];
-                try reflexivity; simpl.
-              simpl; intros ????? H0.
-              unfold rdp_list_is_valid_nonterminal in *.
-              apply list_in_bl in H0; [ | apply @string_bl ]; assumption. }
-            { rewrite !take_long; (assumption || reflexivity). }
-            { apply bool_eq_empty; rewrite drop_length; omega. } } } } }
-    { unfold is_valid_nonterminal in Hvalid; simpl in Hvalid.
-      unfold rdp_list_is_valid_nonterminal in Hvalid; simpl in Hvalid.
-      hnf in Hvalid.
-      apply Equality.list_in_bl in Hvalid; [ | apply @Equality.string_bl ].
-      generalize (@rules_for_complete Char G splitter str _ Hvalid).
-      clear Hvalid.
-      simpl.
-      intros H p.
-      set (prods := G nt) in p.
-      assert (H' : { prefix : _ | prefix ++ prods = G nt }) by (eexists nil; reflexivity).
-      clearbody prods.
-      generalize dependent (G nt); intro Gnt; clear nt; intros.
-      induction p; destruct H' as [prefix H']; subst.
-      { exists (List.length prefix).
-        specialize (H (List.length prefix)).
-        let m := match goal with m : minimal_parse_of_production _ _ _ _ |- _ => constr:m end in
-        pose proof m as m';
-          apply (@parse_of_production__of__minimal_parse_of_production) in m'.
-        destruct m' as [p Hp].
-        specialize (fun H' => H _ H' p).
-        rewrite !nth_error_length_app in H |- *; simpl in *.
-        specialize (H eq_refl).
-        split; [ | eexists; split; [ reflexivity | eassumption ] ].
-        apply H.
-        erewrite <- parse_of_production_respectful_refl.
-        eapply expand_forall_parse_of_production;
-          [ ..
-          | rewrite parse_of_production_respectful_refl; eassumption ].
-        simpl; intros ????? H0.
-        unfold rdp_list_is_valid_nonterminal in *.
-        apply list_in_bl in H0; [ | apply @string_bl ]; assumption. }
-      { specialize_by assumption.
-        apply IHp.
-        eexists (prefix ++ [_]); simpl.
-        rewrite <- List.app_assoc; simpl.
-        reflexivity. } }
+          [ clear IHx
+          | apply IHx;
+            intros; subst; eapply (H' (_::_)); try eassumption; reflexivity ].
+        specialize (H' nil it its eq_refl).
+        hnf.
+        intros [ n [ pit pits ] ]; simpl in * |- .
+        destruct (Compare_dec.le_ge_dec n (length str)).
+        { exists n; repeat split; eauto.
+          specialize (fun pf =>
+                        H' _ pf
+                           (projT1 (parse_of_item__of__minimal_parse_of_item pit))
+                           (projT1 (parse_of_production__of__minimal_parse_of_production pits))).
+          apply H'; eauto.
+          { erewrite <- parse_of_item_respectful_refl.
+            eapply expand_forall_parse_of_item;
+              [ ..
+              | rewrite parse_of_item_respectful_refl;
+                exact (projT2 (parse_of_item__of__minimal_parse_of_item pit)) ];
+              try reflexivity; simpl.
+            simpl; intros ????? H0.
+            unfold rdp_list_is_valid_nonterminal in *.
+            apply list_in_bl in H0; [ | apply @string_bl ]; assumption. }
+          { erewrite <- parse_of_production_respectful_refl.
+            eapply expand_forall_parse_of_production;
+              [ ..
+              | rewrite parse_of_production_respectful_refl;
+                exact (projT2 (parse_of_production__of__minimal_parse_of_production pits)) ];
+              try reflexivity; simpl.
+            simpl; intros ????? H0.
+            unfold rdp_list_is_valid_nonterminal in *.
+            apply list_in_bl in H0; [ | apply @string_bl ]; assumption. } }
+        { exists (length str).
+          specialize (H' (length str) (reflexivity _)).
+          pose proof (fun H => expand_minimal_parse_of_item (str' := take (length str) str) (or_introl (reflexivity _)) (reflexivity _) (or_introl (reflexivity _)) H pit) as pit'; clear pit.
+          pose proof (fun H => expand_minimal_parse_of_production (str' := drop (length str) str) (or_introl (reflexivity _)) (reflexivity _) (or_introl (reflexivity _)) H pits) as pits'; clear pits.
+          refine ((fun ret => let pit'' := pit' (fst (snd ret)) in
+                              let pits'' := pits' (snd (snd ret)) in
+                              ((H' (projT1 (fst (fst ret) pit'')) (projT1 (snd (fst ret) pits'')) (projT2 (fst (fst ret) pit'')) (projT2 (snd (fst ret) pits'')), pit''), pits'')) _); repeat split.
+          { intro p.
+            exists (projT1 (@parse_of_item__of__minimal_parse_of_item Char splitter G _ _ _ _ _ p)).
+            erewrite <- parse_of_item_respectful_refl.
+            eapply expand_forall_parse_of_item;
+              [ ..
+              | rewrite parse_of_item_respectful_refl;
+                exact (projT2 (parse_of_item__of__minimal_parse_of_item p)) ];
+              try reflexivity; simpl.
+            simpl; intros ????? H0.
+            unfold rdp_list_is_valid_nonterminal in *.
+            apply list_in_bl in H0; [ | apply @string_bl ]; assumption. }
+          { intro p.
+            exists (projT1 (@parse_of_production__of__minimal_parse_of_production Char splitter G _ _ _ _ _ p)).
+            erewrite <- parse_of_production_respectful_refl.
+            eapply expand_forall_parse_of_production;
+              [ ..
+              | rewrite parse_of_production_respectful_refl;
+                exact (projT2 (parse_of_production__of__minimal_parse_of_production p)) ];
+              try reflexivity; simpl.
+            simpl; intros ????? H0.
+            unfold rdp_list_is_valid_nonterminal in *.
+            apply list_in_bl in H0; [ | apply @string_bl ]; assumption. }
+          { rewrite !take_long; (assumption || reflexivity). }
+          { apply bool_eq_empty; rewrite drop_length; omega. } } } }
     Grab Existential Variables.
-    reflexivity.
-    reflexivity.
     reflexivity.
     reflexivity.
     reflexivity.
@@ -165,24 +123,10 @@ Section implementation.
     reflexivity.
   Qed.
 
-  Program Definition parser' : Parser G splitter
+  Program Definition parser : Parser G splitter
     := {| has_parse str := parse_nonterminal (G := G) (data := parser_data) str (Start_symbol G);
-          has_parse_sound str Hparse := let p := parse_nonterminal_sound G _ _ Hparse in
-                                        existT _ (projT1 p) ((fun H => _) (projT2 p));
+          has_parse_sound str Hparse := parse_nonterminal_sound G _ _ Hparse;
           has_parse_complete str p Hp := _ |}.
-  Next Obligation.
-  Proof.
-    erewrite <- parse_of_item_respectful_refl.
-    eapply expand_forall_parse_of_item;
-    [ ..
-    | rewrite parse_of_item_respectful_refl; eassumption ].
-    simpl; intros ????? H0.
-    unfold rdp_list_is_valid_nonterminal in *.
-    apply list_in_bl in H0; [ | apply @string_bl ]; assumption.
-    Grab Existential Variables.
-    reflexivity.
-    reflexivity.
-  Qed.
   Next Obligation.
   Proof.
     dependent destruction p.
