src/Parsers/Refinement/SharpenedExpressionParen.v
@@ -20,77 +20,9 @@ Section IndexedImpl.
   Lemma ComputationalSplitter'
   : FullySharpened (string_spec paren_expr_grammar).
   Proof.
-    lazymatch goal with
-     | [ |- FullySharpened _ ]
-       => (eapply FullySharpened_Start)
-    end.
-    eapply SharpenStep;
-  [ solve [ apply FirstStep ] | ].
-    Timeout 5 unfold rindexed_spec, rindexed_spec'.
-    unfold forall_reachable_productions.
-    Timeout 5 simpl expanded_fallback_list'.
-    unfold expanded_fallback_list_rules'.
-    Timeout 5 simpl map.
-    Timeout 5 unfold fold_right at 1.
-    Timeout 5 simpl map.
-    Timeout 5 unfold Operations.enumerate.
-    Timeout 5 unfold all_disjoint.
-    Timeout 5 simpl map.
-    Timeout 5 unfold Operations.disjoint.
-    Timeout 5 simpl map.
-    Timeout 5 unfold fold_right at 1.
-    Timeout 5 unfold fold_right at 1.
-    Timeout 5 unfold fold_right at 1.
-    Timeout 5 unfold fold_right at 1.
-    Timeout 5 simpl andb.
-    Timeout 5 simpl @snd.
-    Timeout 5 unfold If_Then_Else at 4.
-    Timeout 5 simpl @fst.
-    Timeout 5 change (@If_Then_Else ?A false) with (fun (x y : A) => y).
-    Timeout 5 change (@If_Then_Else ?A true) with (fun (x y : A) => x).
-    Timeout 5 cbv beta.
-    Timeout 5 unfold fold_right at 1.
-    Timeout 5 simpl @fst.
-    Timeout 5 simpl @snd.
-    About Equality.list_bin.
-    Timeout 5 change (@Equality.list_bin) with (fun A f a ls => let lb := fun a' => @Equality.list_bin A f a' ls in lb a).
-    Timeout 5 cbv beta.
-    Timeout 5 repeat match goal with
-      | [ |- appcontext[fun a' => @Equality.list_bin ?A ?f a' [?ls]] ]
-        => let c := constr:(fun a' => @Equality.list_bin A f a' [ls]) in
-           let c' := (eval simpl in c) in
-           change c with c'
-    end.
-    Opaque ParserInterface.rules_list_is_complete.
-    Timeout 5 match goal with
-                | [ |- context[(fun dummy => If @?x dummy Then @?y dummy Else _)] ]
-                  => let c := constr:(fun dummy => If_Then_Else (x dummy) (y dummy)) in
-                     let c' := (eval simpl in c) in
-                     idtac
-              end.
-    Timeout 20 simpl.
-
-    Timeout 5 simpl (Equality.list_bin Equality.ascii_beq).
-    Timeout 5 simpl.
-    Timeout 5 unfold If_Then_Else at 11.
-    Timeout 5 simpl (If true Then _ Else _).
-
-    Timeout 5 simpl.
-
-
-
-     | _ => start_honing
-      end
-
     start honing parser using indexed representation.
 
     hone method "splits".
-    {
-      simplify parser splitter.
-      finish honing parser method.
-    }
-
-    hone method "rules".
     {
       simplify parser splitter.
       finish honing parser method.
