Makefile
@@ -97,12 +97,7 @@ QUERYSTRUCTURES_UNMADE_VO := \
 	src/QueryStructure/Implementation/DataStructures/Bags/InvertedIndexBags.vo
 
 PARSERS_UNMADE_VO := \
-	src/Parsers/Refinement/SharpenedAtMostOneNonTerminal.vo \
-	src/Parsers/Refinement/SharpenedABStar.vo \
-	src/Parsers/Refinement/SharpenedExpressionParen.vo \
-	src/Parsers/Refinement/SharpenedExpressionPlus.vo \
 	src/Parsers/Refinement/SharpenedExpressionPlusParen.vo
-# N.B. src/Parsers/Refinement/IndexedAndAtMostOneNonTerminalReflective.v has some admits
 
 FIAT4MONITORS_UNMADE_VO := \
 	src/Fiat4Monitors/HelloWorld/%.vo \
